src/RunTrace.v
@@ -1,5 +1,3 @@
-(* For debugging purposes *)
-
 Require Import Coq.ZArith.BinInt.
 Require Import bbv.WordScope.
 Require Import bbv.DepEqNat.
@@ -8,24 +6,124 @@ Require Import riscv.RiscvBitWidths.
 Require Import riscv.util.Monad.
 Require Import riscv.util.StateMonad.
 Require Import riscv.Decode.
+Require Import riscv.Memory. (* should go before Program because both define loadByte etc *)
 Require Import riscv.Program.
 Require Import riscv.Execute.
 Require Import riscv.util.PowerFunc.
-Require Import riscv.Memory.
+Require Import riscv.Utility.
 Require Import Coq.Lists.List.
 Import ListNotations.
-Require Import riscv.Run.
 
 Section Riscv.
 
   Context {B: RiscvBitWidths}.
 
-  Inductive TraceEvent: Set :=
-  | TraceLoad(addr: Z)(val: word 32)
-  | TraceLoadFailure(addr: Z).
+  Instance A: Alu (word wXLEN) (word wXLEN) := {|
+    zero := $0;
+    one := $1;
+    add := @wplus wXLEN;
+    sub := @wminus wXLEN;
+    mul := @wmult wXLEN;
+    div := @wdiv wXLEN;
+    rem := @wmod wXLEN;
+    signed_less_than a b := if wslt_dec a b then true else false;
+    unsigned_less_than a (b: word wXLEN) := if wlt_dec a b then true else false;
+    signed_eqb := @weqb wXLEN;
+    shiftL w n := wlshift w (Z.to_nat n);
+    signed_shiftR w n := wrshifta w (Z.to_nat n);
+    unsigned_shiftR w n := wrshift w (Z.to_nat n);
+    xor := @wxor wXLEN;
+    or := @wor wXLEN;
+    and := @wand wXLEN;
+  |}.
 
-  Record TraceRiscvMachine := mkTraceRiscvMachine {
-    machineMem: mem 32;
+  (* TODO this is not the way to do it *)
+
+  Instance immmm: IntegralConversion MachineInt (word wXLEN).
+    unfold MachineInt. constructor. apply ZToWord.
+  Defined.
+  Instance immmm': IntegralConversion (word wXLEN) MachineInt.
+    unfold MachineInt. constructor. apply ZToWord || apply wordToZ.
+  Defined.
+  Instance c: Convertible (word wXLEN) (word wXLEN).
+    unfold MachineInt. constructor; apply id || apply ZToWord || apply wordToZ.
+  Defined.
+  Instance ic8: IntegralConversion Int8 (word wXLEN).
+    cbv -[wXLEN]. constructor. intro. destruct H.
+    refine (nat_cast _ _ (sext w (wXLEN - 8))). abstract bitwidth_omega.
+  Defined.
+  Instance ic16: IntegralConversion Int16 (word wXLEN).
+    cbv -[wXLEN]. constructor. intro. destruct H.
+    refine (nat_cast _ _ (sext w (wXLEN - 16))). abstract bitwidth_omega.
+  Defined.
+  Instance ic32: IntegralConversion Int32 (word wXLEN).
+    cbv -[wXLEN]. constructor. intro. destruct H.
+    refine (nat_cast _ _ (sext w (wXLEN - 32))). abstract bitwidth_omega.
+  Defined.
+  Instance ic8': IntegralConversion (word wXLEN) Int8.
+    cbv -[wXLEN]. constructor. intro. constructor.
+    refine (split1 _ (wXLEN - 8) (nat_cast _ _ H)). abstract bitwidth_omega.
+  Defined.
+  Instance ic16': IntegralConversion (word wXLEN) Int16.
+    cbv -[wXLEN]. constructor. intro. constructor.
+    refine (split1 _ (wXLEN - 16) (nat_cast _ _ H)). abstract bitwidth_omega.
+  Defined.
+  Instance ic32': IntegralConversion (word wXLEN) Int32.
+    cbv -[wXLEN]. constructor. intro. constructor.
+    refine (split1 _ (wXLEN - 32) (nat_cast _ _ H)). abstract bitwidth_omega.
+  Defined.
+  Instance ic8u: IntegralConversion Word8 (word wXLEN).
+    cbv -[wXLEN]. constructor. intro. destruct H.
+    refine (nat_cast _ _ (zext w (wXLEN - 8))). abstract bitwidth_omega.
+  Defined.
+  Instance ic16u: IntegralConversion Word16 (word wXLEN).
+    cbv -[wXLEN]. constructor. intro. destruct H.
+    refine (nat_cast _ _ (zext w (wXLEN - 16))). abstract bitwidth_omega.
+  Defined.
+  Instance ic32u: IntegralConversion Word32 (word wXLEN).
+    cbv -[wXLEN]. constructor. intro. destruct H.
+    refine (nat_cast _ _ (zext w (wXLEN - 32))). abstract bitwidth_omega.
+  Defined.
+  Instance icZt: IntegralConversion Z (word wXLEN).
+    unfold MachineInt. constructor. apply ZToWord.
+  Defined.
+  Instance icZu: IntegralConversion Z (word wXLEN).
+    unfold MachineInt. constructor. apply ZToWord.
+  Defined.
+  Instance icut: IntegralConversion (word wXLEN) (word wXLEN).
+    constructor. exact id.
+  Defined.
+  Instance ictu: IntegralConversion (word wXLEN) (word wXLEN).
+    constructor. exact id.
+  Defined.
+
+  Definition MW: MachineWidth (word wXLEN) := MachineWidthInst (Z.of_nat log2wXLEN) (word wXLEN).
+
+  Existing Instance MW.
+
+  Definition Register := Z.
+
+  Definition Register0: Register := 0%Z.
+
+  Instance ZName: NameWithEq := {|
+    name := Z
+  |}.
+
+  Definition run1{M: Type -> Type}{MM: Monad M}{RVS: RiscvState M}: M unit :=
+    pc <- getPC;
+    inst <- loadWord pc;
+    execute (decode (Z.of_nat wXLEN) (Int32ToMachineInt inst));;
+    step.
+
+  Definition run{M: Type -> Type}{MM: Monad M}{RVS: RiscvState M}: nat -> M unit :=
+    fun n => power_func (fun m => run1 ;; m) n (Return tt).
+
+  Inductive TraceEvent: Set :=
+  | TraceLoad(sz: nat)(addr: word wXLEN)(val: SignedWord sz)
+  | TraceLoadFailure(addr: word wXLEN).
+
+  Record RiscvMachine := mkRiscvMachine {
+    machineMem: mem 8;
     registers: Register -> word wXLEN;
     pc: word wXLEN;
     nextPC: word wXLEN;
@@ -33,76 +131,111 @@ Section Riscv.
     executionTrace: list TraceEvent;
   }.
 
-  Definition TODO{T: Type}: T. Admitted.
+  Definition with_machineMem me ma :=
+    mkRiscvMachine me ma.(registers) ma.(pc) ma.(nextPC) ma.(exceptionHandlerAddr) ma.(executionTrace).
+  Definition with_registers r ma :=
+    mkRiscvMachine ma.(machineMem) r ma.(pc) ma.(nextPC) ma.(exceptionHandlerAddr) ma.(executionTrace).
+  Definition with_pc p ma :=
+    mkRiscvMachine ma.(machineMem) ma.(registers) p ma.(nextPC) ma.(exceptionHandlerAddr) ma.(executionTrace).
+  Definition with_nextPC npc ma :=
+    mkRiscvMachine ma.(machineMem) ma.(registers) ma.(pc) npc ma.(exceptionHandlerAddr) ma.(executionTrace).
+  Definition with_exceptionHandlerAddr eh ma :=
+    mkRiscvMachine ma.(machineMem) ma.(registers) ma.(pc) ma.(nextPC) eh ma.(executionTrace).
+  Definition with_executionTrace t ma :=
+    mkRiscvMachine ma.(machineMem) ma.(registers) ma.(pc) ma.(nextPC) ma.(exceptionHandlerAddr) t.
 
-(*
-  Instance IsTraceRiscvMachine: RiscvState (State TraceRiscvMachine) :=
+  Definition liftLoad{sz: nat}(f: mem 8 -> word wXLEN -> option (SignedWord sz))(a: word wXLEN)
+    : State RiscvMachine (SignedWord sz) :=
+    m <- get;
+    match f m.(machineMem) a with
+    | Some v =>
+        put (with_executionTrace (m.(executionTrace) ++ [TraceLoad sz a v]) m);;
+        Return v
+    | None =>
+        put (with_nextPC m.(exceptionHandlerAddr) m);;
+        put (with_executionTrace (m.(executionTrace) ++ [TraceLoadFailure a]) m);;
+        Return (mkSignedWord $0)
+    end.
+
+  Definition liftStore{sz: nat}(f: mem 8 -> word wXLEN -> SignedWord sz -> option (mem 8))
+    (a: word wXLEN)(v: SignedWord sz) : State RiscvMachine unit :=
+    m <- get;
+    match f m.(machineMem) a v with
+    | Some mem' => put (with_machineMem mem' m)
+    | None => put (with_nextPC m.(exceptionHandlerAddr) m)
+    end.
+
+  Instance IsRiscvMachine: RiscvState (State RiscvMachine) :=
   {|
-      getRegister := fun (reg: Register) =>
+      getRegister := fun (reg: name) =>
         if dec (reg = Register0) then
           Return $0
         else
           machine <- get; Return (machine.(registers) reg);
 
-      setRegister := fun (reg: Register) (v: word wXLEN) =>
+      setRegister := fun s ic (reg: name) (v: s) =>
         if dec (reg = Register0) then
           Return tt
         else
           machine <- get;
-          match machine with
-          | mkTraceRiscvMachine imem regs pc npc eh tr =>
-              put (mkTraceRiscvMachine imem 
-                                  (fun reg2 => if dec (reg = reg2) then v else regs reg2)
-                                  pc npc eh tr)
-          end;
+          let newRegs := (fun reg2 => if dec (reg = reg2)
+                                      then (fromIntegral v)
+                                      else machine.(registers) reg2) in
+          put (with_registers newRegs machine);
 
-      getPC := 
-        p <- gets pc;
-        Return (wordToZ p); (* TODO this should be unsigned *)
+      getPC := gets pc;
 
-      setPC := fun (newPC: Z) =>
+      setPC := fun newPC =>
         machine <- get;
-        match machine with
-        | mkTraceRiscvMachine imem regs pc npc eh tr =>
-            put (mkTraceRiscvMachine imem regs pc (ZToWord _ newPC) eh tr)
-        end;
+        put (with_nextPC newPC machine);
 
-      loadByte := TODO;
-      loadHalf := TODO;
+      loadByte   := liftLoad Memory.loadByte;
+      loadHalf   := liftLoad Memory.loadHalf;
+      loadWord   := liftLoad Memory.loadWord;
+      loadDouble := liftLoad Memory.loadDouble;
 
-      loadWord := fun x => 
-        machine <- get;
-        match machine with
-        | mkTraceRiscvMachine imem regs pc npc eh tr =>
-            let addr := (ZToWord 32 (x / 4)) in
-            match read_mem addr imem with
-            | Some v => 
-                put (mkTraceRiscvMachine imem regs pc npc eh (tr ++ [TraceLoad x v]));;
-                Return v
-            | None =>
-                put (mkTraceRiscvMachine imem regs pc npc eh (tr ++ [TraceLoadFailure x]));;
-                Return $0
-            end
-        end;
-
-      loadDouble := TODO;
-
-      storeByte := TODO;
-      storeHalf := TODO;
-      storeWord := TODO;
-      storeDouble := TODO;
+      storeByte   := liftStore Memory.storeByte;
+      storeHalf   := liftStore Memory.storeHalf;
+      storeWord   := liftStore Memory.storeWord;
+      storeDouble := liftStore Memory.storeDouble;
 
       step :=
-        machine <- get;
-        match machine with
-        | mkTraceRiscvMachine imem regs pc npc eh tr =>
-            put (mkTraceRiscvMachine imem regs npc (npc ^+ $4) eh tr)
-        end;
+        m <- get;
+        put (with_nextPC (m.(nextPC) ^+ $4) (with_pc m.(nextPC) m));
+
+      raiseException _ _ :=
+        m <- get;
+        put (with_nextPC m.(exceptionHandlerAddr) m);
   |}.
-*)
+
+  Fixpoint storeWords(l: list (word 32))(a: word wXLEN)(m: mem 8): option (mem 8) :=
+    match l with
+    | nil => Some m
+    | cons w l' =>
+        match Memory.storeWord m a (mkSignedWord w) with
+        | Some m' => storeWords l' (a ^+ $4) m'
+        | None => None
+        end
+    end.
+
+  Definition storeWords_if_mem_accepts(l: list (word 32))(m: mem 8): mem 8 :=
+    match storeWords l $0 m with
+    | Some m' => m'
+    | None => m
+    end.
+
+  (* Puts given program at address 0, and makes pc point to beginning of program, i.e. 0.
+     TODO maybe later allow any address?
+     Note: Keeps the original exceptionHandlerAddr, and the values of the registers,
+     which might contain any undefined garbage values, so the compiler correctness proof
+     will show that the program is correct even then, i.e. no initialisation of the registers
+     is needed. *)
+  Definition putProgram(prog: list (word 32))(m: RiscvMachine): RiscvMachine :=
+    match m with
+    | mkRiscvMachine m regs _ _ eh tr =>
+        mkRiscvMachine (storeWords_if_mem_accepts prog m) regs $0 $4 eh tr
+    end.
 
 End Riscv.
 
-(*
-Existing Instance IsTraceRiscvMachine. (* needed because it was defined inside a Section *)
-*)
+Existing Instance IsRiscvMachine. (* needed because it was defined inside a Section *)
